Added let expressions.  Changed recursions to have separate clauses for defs and def-lists.

LEProps.v
@@ -28,7 +28,7 @@ Import Common LDef LEval.
           term t, when evaluated in runtime-context g, 
           will either yield a value [v] such that [v:::T] or not terminate 
           (but it won't get stuck).
-        - [Fs / g =>:* Ls] (aka [may_exec_list_to Fs g Ls]): 
+        - [Fs / g =>:* Ls] (aka [may_exec_pdefs_to Fs g Ls]): 
           [Fs] is a list of definitions, each [(Fv xi ti)], 
           [Ls] is a list of declarations, each [(Lv xi Ti)], 
           and for each [i], [ti / g =>: Ti]; thus executing [Fs] will 
@@ -37,7 +37,7 @@ Import Common LDef LEval.
         - [result_ok er T]: [er] (an instance of [ef_return]) is either 
           [efr_normal v] and [v ::: T]
           or [er] is [efr_nogas]; [er] is not [efr_stuck].
-        - [result_list_ok xr Ls]: [xr] (an instance of [xf_return]) is either 
+        - [pdefs_result_ok xr Ls]: [xr] (an instance of [xf_return]) is either 
           [efr_normal bs] and [bs :::* Ls]
           or [xr] is [efr_nogas]; [xr] is not [efr_stuck].
 
@@ -63,12 +63,17 @@ Fixpoint value_has_type (v : evalue) (T : ty) {struct T} : Prop :=
     end
   in let may_eval_to (t : tm) (g : rctx) (T : ty) : Prop := 
     forall n, result_ok (evalF t g n) T
+  in let binding_matches_decl
+           (b : vbinding) (L : decl) : Prop :=
+    match (L, b) with
+      | ((Lv x T), (y, v)) => x=y /\ v ::: T
+    end
   in let fix bindings_match_decls 
            (bs : alist evalue) (Ls : list decl) {struct Ls} : Prop :=
     match (Ls, bs) with
       | (nil, nil) => True
-      | ((Lv x T) :: Ls', ((y, v) :: bs')) =>
-          x=y /\ v ::: T /\ bindings_match_decls bs' Ls'
+      | ((L :: Ls'), (b :: bs')) =>
+         binding_matches_decl b L /\ bindings_match_decls bs' Ls'
       | (_, _) => False
     end
   in match (T, v) with
@@ -81,42 +86,63 @@ Fixpoint value_has_type (v : evalue) (T : ty) {struct T} : Prop :=
   end
 where "v ':::' T" := (value_has_type v T).
 
+Definition binding_matches_decl (b: vbinding) (L: decl) : Prop :=
+  match (L, b) with
+    | ((Lv x T), (y, v)) => x=y /\ v ::: T
+  end.
+
 Fixpoint bindings_match_decls 
            (bs : alist evalue) (Ls : list decl) {struct Ls} : Prop :=
     match (Ls, bs) with
       | (nil, nil) => True
-      | ((Lv x T) :: Ls', ((y, v) :: bs')) =>
-          x=y /\ v ::: T /\ bindings_match_decls bs' Ls'
+      | (L :: Ls', (b :: bs')) =>
+          binding_matches_decl b L /\ bindings_match_decls bs' Ls'
       | (_, _) => False
     end.
 Notation "g ':::*' G" := (bindings_match_decls g G).
 
-Definition result_ok (er : ef_return) (T : ty) : Prop :=
+
+Definition res_ok_g
+  {Tv : Type} {Tty : Type} {Rvht : Tv -> Tty -> Prop}
+  (er : ef_return_g Tv) (T : Tty) : Prop :=
     match er with
-      | efr_normal vr => vr ::: T
+      | efr_normal v => Rvht v T
       | efr_nogas => True
       | efr_stuck => False
     end.
 
-Definition result_list_ok (er : xf_return) (Ls : list decl) : Prop :=
-    match er with
-      | efr_normal bs => bs :::* Ls
-      | efr_nogas => True
-      | efr_stuck => False
-    end.
+Definition result_ok : ef_return -> ty -> Prop :=
+  res_ok_g (Rvht:=value_has_type).
+
+Definition vb_result_ok (er : bf_return) (L : decl) : Prop :=
+  res_ok_g (Rvht:=binding_matches_decl) er L.
+
+Definition pdefs_result_ok (er : xf_return) (Ls : list decl) : Prop :=
+  res_ok_g (Rvht:=bindings_match_decls) er Ls.
+
+Definition mevt_g {Ttm : Type} {Tty: Type} {Tv : Type}  
+                  {Fev : Ttm -> rctx -> nat -> (ef_return_g Tv)}
+                  {Rvht : Tv -> Tty -> Prop}
+                  (t : Ttm) (g : rctx) (T : Tty) : Prop := 
+    forall n, res_ok_g (Rvht:=Rvht) (Fev t g n) T.
 
 Definition may_eval_to (t : tm) (g : rctx) (T : ty) : Prop := 
-    forall n, result_ok (evalF t g n) T.
+  mevt_g (Fev:=evalF) (Rvht:=value_has_type) t g T.
 Notation "t '/' g '=>:' T" := (may_eval_to t g T) 
     (at level 40, g at level 39).
 
-Definition may_exec_list_to (Fs : list def) (g : rctx) (Ls : list decl) : Prop := 
-    forall n', result_list_ok (execF_list Fs g n') Ls.
-Notation "Fs '/' g '=>:*' Ls" := (may_exec_list_to Fs g Ls) 
+Definition may_exec_def_to (F : def) (g : rctx) (L : decl) : Prop := 
+  mevt_g (Fev:=execF_def) (Rvht:=binding_matches_decl) F g L.
+
+Definition may_exec_pdefs_to 
+      (Fs : list def) (g : rctx) (Ls : list decl) : Prop := 
+  mevt_g (Fev:=execF_pdefs) (Rvht:=bindings_match_decls) Fs g Ls.
+Notation "Fs '/' g '=>:*' Ls" := (may_exec_pdefs_to Fs g Ls) 
     (at level 40, g at level 39).
 
-Hint Unfold value_has_type bindings_match_decls result_ok result_list_ok 
-     may_eval_to may_exec_list_to.
+Hint Unfold value_has_type binding_matches_decl bindings_match_decls 
+     result_ok vb_result_ok pdefs_result_ok 
+     may_eval_to may_exec_def_to may_exec_pdefs_to mevt_g.
 
 
 (** The following are some alternate definition bodies of [bs:::*Ls] that I've 
@@ -165,7 +191,7 @@ Lemma vht_defs_eq:
   forall v T, value_has_type v T <-> value_has_type' v T.
 Proof.
   intros. split; intro H. 
-    Case "->". induction T; destruct v; simpl in H; auto.
+    Case "->". induction T; destruct v; simpl in H; auto. 
     Case "<-". induction T; destruct v; simpl in H; auto.
 Qed.
 
@@ -173,10 +199,10 @@ Qed.
 (* ###################################################################### *)
 (** ** Lemmas  *)
 (** *** A Lemma for induction on [:::*] *)
-(** Lemma [bmd_ind] is a handy lemma for doing a form of induction over :::*.
+(** Lemma [bmds_ind] is a handy lemma for doing a form of induction over :::*.
     Use it with the [refine] tactic. *)
 
-Lemma bmd_ind: 
+Lemma bmds_ind: 
   forall (P : list decl -> alist evalue -> Type)
     (fnil : P nil nil)
     (fcons: forall x v T Ls' bs', 
@@ -189,7 +215,7 @@ Proof.
     Case "Ls = []". 
       apply fnil.
     Case "Ls = L :: Ls'".
-      destruct Hbmd as (Heq & Hvyt & Hbmd'). subst y. 
+      destruct Hbmd as ([Heq Hvyt] & Hbmd').  subst y. 
       apply (fcons _ _ _ _ _ Hvyt (IHLs' _ Hbmd')).
 Qed.
 
@@ -211,7 +237,7 @@ Lemma VHT_Abs :
   forall xf tb gf T1 T2,
     (forall va,  va ::: T1 -> tb / (aextend xf va gf) =>: T2) ->
     vabs xf tb gf ::: TArrow T1 T2.
-Proof. introv H. simpl. exact H. Qed.
+Proof. introv H. exact H. Qed.
 
 Lemma VHT_Rcd : 
   forall Fs Ls,
@@ -219,17 +245,23 @@ Lemma VHT_Rcd :
     vrcd Fs ::: TRcd Ls.
 Proof. introv H. simpl. exact H. Qed.
 
+Lemma BMD :
+  forall x v T,
+    v ::: T ->
+    binding_matches_decl (x, v) (Lv x T).
+Proof. auto. Qed.
+
 Lemma BMDs_nil :
   nil :::* nil.
 Proof. simpl. constructor. Qed.
 
 Lemma BMDs_cons : 
-  forall G g x v T,
-    g :::* G ->
-    v ::: T ->
-    (aextend x v g) :::* (add_vdecl x T G).
-Proof. auto.
-  introv HgG HvT. simpl. auto. 
+  forall b bs L Ls,
+    binding_matches_decl b L ->
+    bs :::* Ls ->
+    (b :: bs) :::* (L :: Ls).
+Proof.
+  introv Hbmd HgG. simpl. auto. 
 Qed.
 
 Lemma MET:
@@ -237,7 +269,7 @@ Lemma MET:
     (forall n er, evalF t g n = er -> result_ok er T) -> 
     (t / g =>: T).
 Proof.
-  introv H. red. apply (fun n => H n (evalF t g n) eq_refl).
+  introv H. red. red. apply (fun n => H n (evalF t g n) eq_refl).
 Qed.
 
 Lemma ROk_Norm : 
@@ -249,11 +281,11 @@ Proof.
   introv Heq Ht. subst. simpl. exact Ht.
 Qed.
 
-Lemma RLOk_norm : 
-  forall Fs Ls xr,
-    efr_normal Fs = xr ->
-    Fs :::* Ls ->
-    result_list_ok xr Ls.
+Lemma RLOk_Norm: 
+  forall bs Ls xr,
+    efr_normal bs = xr ->
+    bs :::* Ls ->
+    pdefs_result_ok xr Ls.
 Proof.
   introv Heq Ht. subst. simpl. exact Ht.
 Qed.
@@ -292,7 +324,10 @@ Proof.
       assumption.
 Qed.
 
-(** The following isn't accepted by Coq (and isn't really needed):
+(** The following isn't accepted by Coq because Hvt doesn't have a
+    string enough type when passed to the specific inversion functions.
+    It has type [v:::T] while it needs to have a type like [v:::TBool].
+    (However, it isn't really needed):
 <<
   Lemma vht_inversion :
     forall v T (Hvt : v ::: T), 
@@ -346,7 +381,7 @@ Lemma ctxts_agree_on_lookup :
       lookup_vdecl x Ls = Some T ->
         exists v, alookup x bs = Some v /\ v ::: T.
 Proof.
-  refine (bmd_ind _ _ _).
+  refine (bmds_ind _ _ _).
     Case "nil". introv Hlk. inverts Hlk.
     Case "cons". introv Hvt IH Hlk.
       apply lookup_add_vdecl_case in Hlk. 
@@ -402,11 +437,11 @@ Proof.
 Qed.
 
 Lemma ctx_tvar_then_some : forall G x T,
-  G |- (tvar x) \in T -> lookup_vdecl x G = Some T.
+  G |-- (tvar x) \in T -> lookup_vdecl x G = Some T.
 Proof. introv H. inversion H. auto. Qed.
 
 Lemma ctx_tvar_then_alookup : forall G x T g,
-  G |- (tvar x) \in T -> g :::* G -> 
+  G |-- (tvar x) \in T -> g :::* G -> 
     exists v, alookup x g = Some v /\ v ::: T.
 Proof. 
   introv HG Hg. 
@@ -414,7 +449,7 @@ Proof.
 Qed.
 
 Lemma ctx_tvar_then_evalsto : forall G x T g,
-  G |- (tvar x) \in T -> g :::* G -> (tvar x) / g =>: T.
+  G |-- (tvar x) \in T -> g :::* G -> (tvar x) / g =>: T.
 Proof. 
   introv HG Hg. destruct (ctx_tvar_then_alookup G x T g HG Hg) as [v [Hl Hv]].
   unfold may_eval_to. intro n. destruct n as [ | n' ]; simpl; auto.
@@ -423,7 +458,7 @@ Qed.
 
 (** *** Lemmas for more easily proving [t / g =>: T] and [Fs / g  =>:* Ls] *)
 (** These lemmas rearrange things so that the calls to [evalF] and 
-    [execF_list] are in hypotheses such that [let_val] and associates 
+    [execF_pdefs] are in hypotheses such that [let_val] and associates 
     can be applied to them.*)
 
 Lemma evalF_parts :
@@ -437,14 +472,16 @@ Proof.
     apply (H n' _ eq_refl).
 Qed.
 
-Lemma execF_list_parts :
-  forall (Fs : list def) (Ls : list decl) (g : rctx),
-    (forall n' er, execF_list Fs g n' = er -> result_list_ok er Ls) ->
-        Fs / g  =>:* Ls.
+Lemma eF_parts_g {Ttm : Type} {Tty: Type} {Tv : Type} 
+                 {Fev : Ttm -> rctx -> nat -> (ef_return_g Tv)}
+                 {Rvht : Tv -> Tty -> Prop}:
+(*               {Rmet : Ttm -> rctx -> Tty -> Prop}:*)
+  forall (t : Ttm) (T : Tty) (g : rctx),
+    (forall n' er, Fev t g n' = er -> res_ok_g (Rvht:=Rvht) er T) ->
+        mevt_g (Fev:=Fev) (Rvht:=Rvht) t g T.
 Proof.
   exact (fun _ _ _ H n' => H n' _ eq_refl).
 Qed.
-
 
 (** *** Lemmas for reasoning about LETRT forms. *)
 (** These lemmas are for reasoning about [LETRT] forms.
@@ -453,86 +490,39 @@ Qed.
     subgoals that reason about the let- and in- clauses.
 
     Because [LETRT] is a notation, it is essentially generic in that it can 
-    be used with both [evalF] and [execF_list].  Also the IN clause can be 
+    be used with both [evalF] and [execF_pdefs].  Also the IN clause can be 
     either a singelton or a list.  However, lemmas are not notations,
     so there are four lemmas to handle the different cases. *)
 
-Lemma let_val : 
-  forall t1 g n' (f : evalue -> ef_return) erf T1 T2,
-    (LETRT x <== evalF t1 g n' IN f x) = erf ->
-    t1 / g =>: T1 -> 
+Lemma let_ok_g
+     {Ttm1 : Type} {Tty1: Type} {Tv1 : Type}  
+     {Fev1 : Ttm1 -> rctx -> nat -> (ef_return_g Tv1)}
+     {Rvht1 : Tv1 -> Tty1 -> Prop}
+     {Tv2 : Type} {Tty2 : Type} {Rvht2: Tv2 -> Tty2 -> Prop}:  
+  let Ter2 := ef_return_g Tv2 in
+  let Rrok := res_ok_g (Rvht:=Rvht2) in
+  forall {t1} {g} {n'} {f : Tv1 -> Ter2} {erf : Ter2} {T1} {T2 : Tty2},
+    (LETRT v <== Fev1 t1 g n' IN f v) = erf ->
+    mevt_g (Fev:=Fev1) (Rvht:=Rvht1) t1 g T1 -> 
     (forall v1, 
-       v1 ::: T1 -> 
-       forall er2, 
+       Rvht1 v1 T1 -> 
+       forall (er2 : Ter2), 
          (f v1) = er2 -> 
-         result_ok er2 T2) -> 
-    result_ok erf T2.
+         Rrok er2 T2) -> 
+    Rrok erf T2.
 Proof. 
     introv HLet Heval Hin. 
     specialize (Heval n'). 
-    destruct (evalF t1 g n') as [v1 | | ]; try (subst erf; auto; fail).
-      Case "result_ok v1". 
-        unfold result_ok in Heval. 
+    destruct (Fev1 t1 g n') as [v1 | | ]; try (subst erf; auto; fail).
+      Case "efr_normal v1". 
         apply (Hin v1 Heval erf HLet).
 Qed.
 
-Lemma let_vlist : 
-  forall Fs g n' (f : alist evalue -> ef_return) erf Ls T2,
-    (LETRT bs <== execF_list Fs g n' IN f bs) = erf ->
-    Fs / g =>:* Ls -> 
-    (forall bs1,
-       bs1 :::* Ls -> 
-       forall er2, 
-         (f bs1) = er2 -> 
-         result_ok er2 T2) -> 
-    result_ok erf T2.
-Proof. 
-    introv HLet Heval Hin. 
-    specialize (Heval n'). 
-    destruct (execF_list Fs g n') as [bs1 | | ]; try (subst erf; auto; fail).
-      Case "result_list_ok bs1". 
-        unfold result_list_ok in Heval. 
-        apply (Hin bs1 Heval erf HLet).
-Qed.
-
-Lemma list_let_val : 
-  forall t1 g n' (f : evalue -> xf_return) xrf T1 T2,
-    (LETRT x <== evalF t1 g n' IN f x) = xrf ->
-    t1 / g =>: T1 -> 
-    (forall v1,
-       v1 ::: T1 -> 
-       forall er2, 
-         (f v1) = er2 -> 
-         result_list_ok er2 T2) -> 
-    result_list_ok xrf T2.
-Proof. 
-    introv HLet Heval Hin. 
-    specialize (Heval n'). 
-    destruct (evalF t1 g n') as [v1 | | ]; try (subst xrf; auto; fail).
-      Case "result_ok v1". 
-        unfold result_ok in Heval. 
-        apply (Hin v1 Heval xrf HLet).
-Qed.
-
-Lemma list_let_vlist : 
-  forall Fs1 g n' (f : alist evalue -> xf_return) erf Ls1 Ls2,
-    (LETRT bs1 <== execF_list Fs1 g n' IN f bs1) = erf ->
-    Fs1 / g =>:* Ls1 -> 
-    (forall bs1,
-       bs1 :::* Ls1 -> 
-       forall er2, 
-         (f bs1) = er2 -> 
-         result_list_ok er2 Ls2) -> 
-    result_list_ok erf Ls2.
-Proof. 
-    introv HLet Heval Hin. 
-    specialize (Heval n'). 
-    destruct (execF_list Fs1 g n') as [bs1 | | ]; try (subst erf; auto; fail).
-      Case "result_list_ok bs1". 
-        unfold result_list_ok in Heval. 
-        apply (Hin bs1 Heval erf HLet).
-Qed.
-
+(* Call this on 
+   evalue ty value_has_type
+   vbinding decl binding_matches_decl
+   (alist evalue) (list decl) bindings_match_decls
+*)
 
 (* ###################################################################### *)
 (**  ** Proof of soundness of evalF *)
@@ -544,22 +534,26 @@ Qed.
    The proof is by induction on [t] using the custom induction principle
    so that records are handled correctly.  For each case, the typing relation
    is inverted to yield type assertions about the components of [t] and
-   [evalF_parts] (or [execF_list_parts]) and [simpl] are applied ending
+   [evalF_parts] (or [execF_pdefs_parts]) and [simpl] are applied ending
    up with the appropriate clause of [evalF] in [Hev].
 *) 
 
-  
+
+
 Theorem evalF_is_sound_yielding_T : 
   forall (t : tm) (G : context) (T : ty) (g : rctx),
-    G |- t \in T ->  g :::* G -> t / g  =>: T.
+    G |-- t \in T ->  g :::* G -> t / g  =>: T.
 Proof.
-  set (Q:=fun Fs : list def =>
+  set (Q:=fun F : def =>
+          forall (G : context) (L : decl) (g : rctx),
+            def_yields G F L ->  g :::* G -> may_exec_def_to F g L).
+  set (QL:=fun Fs : list def =>
           forall (G : context) (Ls : list decl) (g : rctx),
-            G |- Fs *\in Ls ->  g :::* G -> Fs / g  =>:* Ls).
-  tm_xind_tactic t Q Case; 
+            G |-- Fs *\in Ls ->  g :::* G -> Fs / g  =>:* Ls).
+  tm_xind_tactic t Q QL Case; 
     introv Hty HGg; inverts Hty; 
-    (apply evalF_parts || apply execF_list_parts);
-    intros n' er Hev; simpl in Hev; subst Q.
+    (apply evalF_parts || apply eF_parts_g);
+    intros n' er Hev; simpl in Hev; subst Q QL.
 
   Case "ttrue". 
     exact (ROk_Norm _ _ _ Hev VHT_True).
@@ -571,62 +565,64 @@ Proof.
     destruct (ctxts_agree_on_lookup _ _ HGg _ _ H1) as [v [Hlk Hvt]].
     rewrite Hlk in Hev. exact (ROk_Norm _ _ _ Hev Hvt).
 
+  Case "tabs". 
+    apply (ROk_Norm _ _ _ Hev); clear Hev.
+    apply VHT_Abs; intros va Hvat.
+    apply (IHtb _ _ _ H4); clear IHtb H4.
+    apply (BMDs_cons _ _ _ _ (BMD _ _ _ Hvat) HGg). 
+
   Case "tapp".
     (* use IHs to get [Ht1 : t1 / g =>: TArrow T11 T] & [Ht2 : t2 / g =>: T11].  *)
     assert (Ht1 := IHt1 _ _ _ H2 HGg); clear IHt1 H2.
     assert (Ht2 := IHt2 _ _ _ H4 HGg); clear IHt2 H4.
     (* use the [let_val] lemma with Ht1 and Ht2 to decompose the two LETRT forms *)
-    apply (let_val t1 g n' _ _ _ T Hev Ht1); clear Hev Ht1;
-    intros v1 Hv1t erL2 HevL2.
-    apply (let_val t2 g n' _ _ _ _ HevL2 Ht2); clear HevL2 Ht2;
-    intros v2 Hv2t erf Hevf.
-    assert (Hex := vht_inv_arrow _ _ _ Hv1t); clear Hv1t;
-    destruct Hex as (xf & tb & gf & Hv1eq & Hva); subst v1 erf.
+    apply (let_ok_g Hev Ht1); clear Hev Ht1; intros v1 Hv1t erL2 HevL2.
+    destruct (vht_inv_arrow _ _ _ Hv1t) as (xf & tb & gf & -> & Hva); clear Hv1t. 
+    apply (let_ok_g HevL2 Ht2); clear HevL2 Ht2; intros v2 Hv2t ? <-.
     apply (Hva v2 Hv2t n').
 
-  Case "tabs". 
-    apply (ROk_Norm _ _ _ Hev); clear Hev.
-    apply VHT_Abs; intros va Hvat.
-    apply (IHtb _ _ (aextend x va g) H4). clear IHtb.
-    apply (BMDs_cons _ _ _ _ _ HGg Hvat).
-
   Case "trcd". 
-    rewrite <- (execF_list_eq Fs g n') in Hev.
+    rewrite <- (execF_pdefs_eq Fs _ n') in Hev.
     assert (HFs := IHFs _ _ _ H1 HGg); clear IHFs H1.
-    apply (let_vlist _ g n' _ _ _ _ Hev HFs); clear Hev HFs;
-    intros bs Hbst er2 Hev2. 
+    apply (let_ok_g Hev HFs); clear Hev HFs; intros bs Hbst er2 Hev2. 
     apply (ROk_Norm _ _ _ Hev2 (VHT_Rcd _ _ Hbst)).
-
-  Case "trnil".
-    apply (RLOk_norm _ _ _ Hev BMDs_nil). 
-
-  Case "trcons".
-    assert (Ht := IHt _ _ _ H4 HGg); clear IHt H4.
-    assert (HFs := IHFs _ _ _ H5 HGg); clear IHFs H5.
-    apply (list_let_val tx g n' _ _ T _ Hev Ht); clear Hev Ht;
-    intros v1 Hv1t erL2 HevL2.
-    apply (list_let_vlist _ g n' _ _ Tr _ HevL2 HFs); clear HevL2 HFs;
-    intros bs2 Hbs2t erf Hevf. 
-    apply (RLOk_norm _ _ _ Hevf).
-    apply (BMDs_cons _ _ _ _ _ Hbs2t Hv1t).
 
   Case "tproj". 
     assert (Htr := IHtr _ _ _ H2 HGg); clear IHtr H2.
-    apply (let_val tr g n' _ _ _ _ Hev Htr); clear Hev Htr; 
-    intros vr Hvrt erp Hevp.
-    destruct (vht_inv_rcd _ _ Hvrt) as [bs [? HbsT ]]. subst vr.
+    apply (let_ok_g Hev Htr); clear Hev Htr; intros vr Hvrt erp Hevp.
+    destruct (vht_inv_rcd _ _ Hvrt) as [bs [-> HbsT ]]. 
     destruct (ctxts_agree_on_lookup _ _ HbsT _ _ H4) as [v [Hlk HvT]].
     rewrite Hlk in Hevp. 
     apply (ROk_Norm _ _ _ Hevp HvT).
 
   Case "tif".
     assert (Hti := IHti _ _ _ H3 HGg); clear IHti H3.
-    apply (let_val ti g n' _ _ _ _ Hev Hti); clear Hev Hti;
-    intros vi Hvit erc Hevc.
+    apply (let_ok_g Hev Hti); clear Hev Hti; intros vi Hvit erc Hevc.
     destruct (vht_inv_bool vi Hvit); subst.
       SSCase "v = vtrue". apply (IHtt _ _ _ H5 HGg n').
       SSCase "v = vfalse". apply (IHte _ _ _ H6 HGg n').
 
+  Case "tlet".
+    rewrite <- (execF_def_eq F _ n') in Hev.
+    assert (HF := IHF _ _ _ H2 HGg); clear IHF H2.
+    apply (let_ok_g Hev HF); clear Hev HF; intros b1 Hb1L ? <-. 
+    apply (IHt _ _ (b1::g) H4 (BMDs_cons _ _ _ _ Hb1L HGg)); clear IHt H4.
+
+  Case "F_v".
+    assert (Ht := IHt _ _ _ H3 HGg); clear IHt H3.
+    apply (let_ok_g Hev Ht); clear Hev Ht; intros v1 Hv1T ? <-. 
+    apply (BMD _ _ _ Hv1T).
+
+  Case "Fs_nil".
+    apply (RLOk_Norm _ _ _ Hev BMDs_nil). 
+
+  Case "Fs_cons".
+    assert (HF := IHF _ _ _ H2 HGg); clear IHF H2.
+    assert (HFs := IHFs _ _ _ H4 HGg); clear IHFs H4.
+    apply (let_ok_g Hev HF); clear Hev HF; intros b1 Hb1L er2 Hev2.
+    apply (let_ok_g Hev2 HFs); clear Hev2 HFs; intros bs2 Hbs2t erf Hevf. 
+    apply (RLOk_Norm _ _ _ Hevf).
+    apply (BMDs_cons _ _ _ _ Hb1L Hbs2t). 
 Qed.
 
 (**  *** Proof of [evalF_is_sound] *)
@@ -634,7 +630,7 @@ Qed.
 
 Corollary evalF_is_sound: 
   forall (t : tm) (G : context) (T : ty) (g : rctx) (n : nat),
-    G |- t \in T ->  g :::* G -> evalF t g n  <> efr_stuck.
+    G |-- t \in T ->  g :::* G -> evalF t g n  <> efr_stuck.
 Proof.
   introv Hty HGg.
   assert (Hr := evalF_is_sound_yielding_T _ _ _ _ Hty HGg n).
