XLEval.v
@@ -1,0 +1,127 @@
+(** ** An experiment using extended recursion to define [Eval] *)
+
+(**
+    This file contains an attempt at using the extended induction principle 
+    for terms to define the [eval] function.  Since it recurses on the 
+    structure of terms, it doesn't need the notion of gas (until we add recursion).
+
+   It works pretty well until we get to [tapp]: we can get [v1] and [v2] and
+   turn [v2] into [(vabs x t gf)] but there's no way to evaluate [t]
+   since there's no direct access to [eval].
+
+   However, the [tabs x T t] branch has [ev_t] which is essentially [(eval t)].
+   So what we want is to store ev_t in [vabs] instead of the raw term, [t].
+   But the type of [ev_t] is [(valist -> nat -> ef_return)] which runs into the
+   "Non strictly positive occurrence" prohibition because [valist] is to the left of
+   an arrow.  Variations with [value] or [vbinding] to the left also don't work.
+*)
+
+
+Load Init.
+Require Export SfLib.
+Require Import LibTactics.
+
+Require Export Common LDef.
+Import Common LDef.
+
+Inductive ef_return_g (Tr : Type) :  Type :=
+  | efr_normal : Tr -> ef_return_g Tr
+  | efr_nogas : ef_return_g Tr
+  | efr_stuck : ef_return_g Tr.
+
+Arguments efr_normal [Tr] _.
+Arguments efr_nogas [Tr].
+Arguments efr_stuck [Tr].
+
+
+Inductive value : Type :=
+  | vid : id -> value
+  | vabs : id -> (valist -> nat -> ef_return_g value) -> valist -> value
+  | vtrue : value
+  | vfalse : value
+  | vrcd : valist -> value
+with vbinding : Type :=
+  | vbF : id -> value -> vbinding
+with valist : Type :=
+  | vl_nil : valist
+  | vl_cons : vbinding -> valist -> valist.
+
+
+Definition ef_return := ef_return_g value.
+Definition bf_return := ef_return_g vbinding.
+Definition xf_return := ef_return_g valist.
+
+
+Notation "'LETRT' x <== er1 'IN' er2" 
+   := (match er1 with
+         | efr_normal x => er2
+         | efr_nogas => efr_nogas
+         | efr_stuck => efr_stuck
+       end)
+   (right associativity, at level 60).
+
+Fixpoint alookup (x: id) (a: valist) : option value :=
+  match a with
+    | vl_nil => None
+    | vl_cons (vbF y v) a' => 
+        if eq_id_dec y x then (Some v) else (alookup x a')
+    end.
+
+Definition eval_tmf : tm -> valist -> nat -> ef_return :=
+  tm_xrect 
+    (*P*)    (fun _ => valist -> nat -> ef_return)
+    (*Q*)    (fun _ => valist -> nat -> bf_return)
+    (*QL*)   (fun _ => valist -> nat -> xf_return)
+    (* ttrue *) (fun _ _ => efr_normal vtrue)
+    (* ttfalse *) (fun _ _ => efr_normal vfalse)
+    (* tvar *) (fun x g n' => 
+                  match alookup x g with 
+                    | Some v => efr_normal v 
+                    | None => efr_stuck 
+                  end)
+    (* tabs *) (fun x T t ev_t g n' => 
+                  efr_normal (vabs x (ev_t vl_nil) g))
+    (* tapp *) (fun t1 ef_t1 t2 ef_t2 g n' =>
+                  LETRT v1 <== ef_t1 g n' IN
+                    LETRT v2 <== ef_t2 g n' IN
+                      match v1 with 
+                        | vabs x tf te => 
+                            tf (* (vl_cons (vbF x v2) te) *) n' 
+                        | _ => efr_stuck
+                      end)
+    (* trcd *) (fun Fs ef_Fs g n' => 
+                  LETRT bs <== ef_Fs g n' IN efr_normal (vrcd bs))
+    (* tproj *) (fun t ef_t x g n' => 
+                  LETRT v <== ef_t g n' IN
+                    match v with
+                      | vrcd bs => match alookup x bs with
+                                     | Some v => efr_normal v
+                                     | _ => efr_stuck
+                                   end
+                      | _ => efr_stuck
+                    end)
+      (* tif *) (fun tb ef_tb tt ef_tt te ef_te g n' => 
+                  LETRT vb <== ef_tb g n' IN
+                    match vb with
+                      | vtrue => ef_tt g n'
+                      | vfalse => ef_te g n'
+                      | _ => efr_stuck
+                    end)
+      (* tlet *) (fun F ef_F t2 ef_t2 g n' => 
+                  LETRT b <== ef_F g n' IN
+                    ef_t2 (vl_cons b g) n')
+      (* Fv *) (fun x t ef_t g n' => 
+                  LETRT v <== ef_t g n' IN 
+                    efr_normal (vbF x v))
+      (* nil *) (fun _ _ => efr_normal vl_nil)
+      (* cons *) (fun F ef_F Fs' ef_Fs' g n' => 
+                  LETRT b <== ef_F g n' IN
+                    LETRT bs' <== ef_Fs' g n' IN 
+                      efr_normal (vl_cons b bs')).
+
+
+Fixpoint evalF (t : tm) (g : valist) (n : nat) : ef_return :=
+  match n with
+    | O => efr_nogas
+    | S n' => eval_tmf t g n'
+  end.
